src/HOL/IMP/Abs_Int2_ivl.thy
@@ -248,27 +248,25 @@ qed
 
 subsubsection "Tests"
 
-value "show_acom (the(AI_ivl test1_ivl))"
+value "show_acom_opt (AI_ivl test1_ivl)"
 
 text{* Better than @{text AI_const}: *}
-value "show_acom (the(AI_ivl test3_const))"
-value "show_acom (the(AI_ivl test4_const))"
-value "show_acom (the(AI_ivl test6_const))"
+value "show_acom_opt (AI_ivl test3_const)"
+value "show_acom_opt (AI_ivl test4_const)"
+value "show_acom_opt (AI_ivl test6_const)"
 
-definition "steps c i = (step_ivl(top c) ^^ i) (bot c)"
+definition "steps c i = (step_ivl(top(vars c)) ^^ i) (bot c)"
 
-value "test2_ivl"
-value "show_acom (the(AI_ivl test2_ivl))"
+value "show_acom_opt (AI_ivl test2_ivl)"
 value "show_acom (steps test2_ivl 0)"
 value "show_acom (steps test2_ivl 1)"
 value "show_acom (steps test2_ivl 2)"
 value "show_acom (steps test2_ivl 3)"
 
-text{* Fixed point reached in 3 steps.
+text{* Fixed point reached in 2 steps.
  Not so if the start value of x is known: *}
 
-value "test3_ivl"
-value "show_acom (the(AI_ivl test3_ivl))"
+value "show_acom_opt (AI_ivl test3_ivl)"
 value "show_acom (steps test3_ivl 0)"
 value "show_acom (steps test3_ivl 1)"
 value "show_acom (steps test3_ivl 2)"
@@ -281,15 +279,12 @@ loop did not terminate. Worse still, as the following example shows: even if
 the actual execution terminates, the analysis may not. The value of y keeps
 decreasing as the analysis is iterated, no matter how long: *}
 
-value "test4_ivl"
 value "show_acom (steps test4_ivl 50)"
 
 text{* Relationships between variables are NOT captured: *}
-value "test5_ivl"
-value "show_acom (the(AI_ivl test5_ivl))"
+value "show_acom_opt (AI_ivl test5_ivl)"
 
 text{* Again, the analysis would not terminate: *}
-value "test6_ivl"
 value "show_acom (steps test6_ivl 50)"
 
 end
